src/int63/CnfInt63.v
@@ -95,14 +95,24 @@ Section Checker.
     | a::b::c => a::(clean c)
     end.
 
-  Definition check_BuildDefInt lits :=
+(* * and_neg          : {(and a_1 ... a_n) (not a_1) ... (not a_n)}
+     * or_pos           : {(not (or a_1 ... a_n)) a_1 ... a_n} 
+     * implies_pos      : {(not (implies a b)) (not a) b}
+     * xor_pos1         : {(not (xor a b)) a b}
+     * xor_neg1         : {(xor a b) a (not b)}
+     * equiv_pos1       : {(not (iff a b)) a (not b)}
+     * equiv_neg1       : {(iff a b) (not a) (not b)}
+     * ite_pos1         : {(not (if_then_else a b c)) a c}
+     * ite_neg1         : {(if_then_else a b c) a (not c)} *)
+
+  Definition check_BuildDefInt lits i :=
     let n := PArray.length lits in
     match get_form (Lit.blit (lits.[0])) with
     | Fatom a => 
       match get_atom a with
       | Abop b h1 h2 => 
-        match (b,get_atom h1,get_atom h2) with
-        | (BO_eq t,Acop (CO_int x),Acop (CO_int y)) => 
+        match (b) with
+        | (BO_eq Typ.Tint) => 
           let test_correct i0 l :=
             if i0 == 0
             then Lit.is_pos l
@@ -112,11 +122,7 @@ Section Checker.
                 match (get_form (Lit.blit l1),get_form (Lit.blit l2)) with
                 | (Fatom a1,Fatom a2) =>
                   match (get_atom a1,get_atom a2) with
-                  | (Auop (UO_index j) hx1,Auop (UO_index k) hy1) => 
-                    match (get_atom hx1,get_atom hy1) with
-                    | (Acop (CO_int x1),Acop (CO_int y1)) => (Lit.is_pos l1)&&(Lit.is_pos l2)&&(negb (Lit.is_pos l))&&(j == i0-1)&&(k == j)&&(x == x1)&&(y==y1)
-                    | _ => false
-                    end
+                  | (Auop (UO_index j) h1',Auop (UO_index k) h2') => (Lit.is_pos l1)&&(Lit.is_pos l2)&&(negb (Lit.is_pos l))&&(j == i0-1)&&(k == j)&&(h1 == h1')&&(h2'==h2)
                   | _ => false
                   end
                 | _ => false
@@ -125,16 +131,43 @@ Section Checker.
               end
                  )
           in
-          if (n == Int63Op.digits + 1)&&(Lit.is_pos (lits.[0]))&&(Typ.eqb t Typ.Tint)&&forallbi (fun i l => test_correct i l) lits
+          if (n == Int63Op.digits + 1)&&(Lit.is_pos (lits.[0]))&&forallbi (fun i6 l => test_correct i6 l) lits
           then PArray.to_list lits
           else C._true
         | _ => C._true
         end
+      | Auop (UO_index i1) hxor =>
+        match get_atom hxor with
+        | Abop b h1 h2 =>
+          match (b) with
+          | (BO_int_xor) =>
+            if n == 3
+            then (
+              match (get_form (Lit.blit (lits.[1])),get_form (Lit.blit (lits.[2]))) with
+              | (Fatom a1,Fatom a2) =>
+                match (get_atom a1,get_atom a2) with
+                | (Auop (UO_index i2) h1', Auop (UO_index i3) h2') => 
+                  if (h1' == h1)&&(h2 == h2')&&(i1 ==i2)&&(i2 == i3)&&(i == i1)&&(Lit.is_pos (lits.[1]))&&(Lit.is_pos (lits.[2]))
+                  then (
+                    if (Lit.is_pos (lits.[0]))
+                    then lits.[0]::lits.[1]::(Lit.neg (lits.[2]))::nil
+                    else lits.[0]::lits.[1]::lits.[2]::nil
+                       )
+                  else C._true   
+                | _ => C._true
+                end
+              | _ => C._true
+              end
+                 )
+            else C._true
+          | _ => C._true
+          end
+        | _ => C._true
+        end
       | _ => C._true
       end
-    | _ => C._true
-    end
-  .
+   | _ => C._true
+   end.
 
 
   Definition check_BuildProjInt lits i :=
@@ -250,38 +283,38 @@ Section Checker.
     Proof.
       unfold check_BuildProjInt,C.valid. intros lits i.
       
-      case_eq (t_form.[Lit.blit (lits.[0])]);intros; auto using C.interp_true.
-      case_eq (t_atom.[i0]);intros; auto using C.interp_true.
-      case_eq b;intros; auto using C.interp_true.
-      case_eq (t_atom.[i1]);intros; auto using C.interp_true.
-      case_eq c;intros; auto using C.interp_true.
-      case_eq (t_atom.[i2]);intros; auto using C.interp_true.
-      case_eq c0;intros; auto using C.interp_true.
-      case_eq (t_form.[Lit.blit (lits.[i+1])]);intros;auto using C.interp_true.
-      case_eq (t_form.[Lit.blit i5]);intros;auto using C.interp_true.
-      case_eq (t_form.[Lit.blit i6]);intros;auto using C.interp_true.
-      case_eq (t_atom.[i7]);intros;auto using C.interp_true.
-      case_eq u;intros;auto using C.interp_true.
-      case_eq (t_atom.[i8]);intros;auto using C.interp_true.
-      case_eq u0;intros;auto using C.interp_true.
-      case_eq (t_atom.[i9]);intros;auto using C.interp_true.
-      case_eq c1;intros;auto using C.interp_true.
-      case_eq (t_atom.[i11]);intros;auto using C.interp_true.
-      case_eq c2;intros;auto using C.interp_true.
+      case_eq (t_form.[Lit.blit (lits.[0])]);intros i0; auto using C.interp_true.
+      case_eq (t_atom.[i0]);intros b; auto using C.interp_true.
+      case_eq b; intros t H i1 i2 H0; auto using C.interp_true; intro H1.
+      case_eq (t_atom.[i1]);intros c H2; auto using C.interp_true.
+      case_eq c;intros i3; auto using C.interp_true; intro H3.
+      case_eq (t_atom.[i2]);intros c0 H4; auto using C.interp_true.
+      case_eq c0;intro i4; auto using C.interp_true;intro H5.
+      case_eq (t_form.[Lit.blit (lits.[i+1])]);intros i5;auto using C.interp_true;intros i6 H6.
+      case_eq (t_form.[Lit.blit i5]);intro i7;auto using C.interp_true;intro H7.
+      case_eq (t_form.[Lit.blit i6]);intro i8;auto using C.interp_true; intro H8.
+      case_eq (t_atom.[i7]);intros u i9;auto using C.interp_true; intros H9.
+      case_eq u;intro i10;auto using C.interp_true;intro H10.
+      case_eq (t_atom.[i8]);intros u0 i11;auto using C.interp_true;intro H11.
+      case_eq u0;intro i12;auto using C.interp_true;intro H12.
+      case_eq (t_atom.[i9]);intros c1 H13;auto using C.interp_true.
+      case_eq c1;intros i13;auto using C.interp_true; intro H14.
+      case_eq (t_atom.[i11]);intros c2 H15;auto using C.interp_true.
+      case_eq c2;intro i14;auto using C.interp_true;intro H16.
 
-      case_eq ((length lits == digits + 1) && (i < digits) && Lit.is_pos i5 && Lit.is_pos i6 && negb (Lit.is_pos (lits .[ 0])) && Lit.is_pos (lits .[ i + 1]) && Typ.eqb t Typ.Tint && (i10 == i) && (i12 == i10) && (i3 == i13) && (i4 == i14));intros.
-      apply andb_true_iff in H17; destruct H17; apply andb_true_iff in H17; destruct H17; apply andb_true_iff in H17; destruct H17; apply andb_true_iff in H17; destruct H17; apply andb_true_iff in H17; destruct H17; apply andb_true_iff in H17; destruct H17; apply andb_true_iff in H17; destruct H17; apply andb_true_iff in H17; destruct H17; apply andb_true_iff in H17; destruct H17; apply andb_true_iff in H17; destruct H17.
+      case_eq ((length lits == digits + 1) && (i < digits) && Lit.is_pos i5 && Lit.is_pos i6 && negb (Lit.is_pos (lits .[ 0])) && Lit.is_pos (lits .[ i + 1]) && Typ.eqb t Typ.Tint && (i10 == i) && (i12 == i10) && (i3 == i13) && (i4 == i14));intro H17.
+      apply andb_true_iff in H17; destruct H17 as (H17,H18); apply andb_true_iff in H17; destruct H17 as (H17,H19); apply andb_true_iff in H17; destruct H17 as (H17,H20); apply andb_true_iff in H17; destruct H17 as (H17,H21); apply andb_true_iff in H17; destruct H17 as (H17,H22); apply andb_true_iff in H17; destruct H17 as (H17,H23); apply andb_true_iff in H17; destruct H17 as (H17,H24); apply andb_true_iff in H17; destruct H17 as (H17,H25); apply andb_true_iff in H17; destruct H17 as (H17,H26); apply andb_true_iff in H17; destruct H17 as (H17,H27).
       
       rewrite Int63Properties.eqb_spec in H19; rewrite Int63Properties.eqb_spec in H20; rewrite Int63Properties.eqb_spec in H21; rewrite Int63Properties.eqb_spec in H18;apply Typ.eqb_spec in H22;subst i10; subst i12; subst i13; subst i14;subst t.
       rewrite <- H3 in H14; rewrite <- H5 in H16; rewrite <- H10 in H12;subst u0; subst c1; subst c2.
       rewrite negb_true_iff in H24.
       
       simpl; rewrite orb_false_r; apply orb_true_iff.
-      unfold Lit.interp; rewrite H24; rewrite H23; rewrite negb_true_iff; unfold Var.interp; rewrite !rho_interp; rewrite H6; rewrite H.
+      unfold Lit.interp; rewrite H24; rewrite H23; rewrite negb_true_iff; unfold Var.interp; rewrite !rho_interp; rewrite H6; rewrite H1.
       simpl; unfold Lit.interp; rewrite H25; rewrite H26; unfold Var.interp; rewrite !rho_interp; rewrite H8; rewrite H7;simpl.
       unfold Atom.interp_form_hatom; unfold interp_hatom; rewrite !t_interp_wf. 
       rewrite H0; rewrite H9;rewrite H11; simpl; rewrite !t_interp_wf.
-      unfold interp_uop; unfold interp_bop; rewrite H10; rewrite H1; simpl; rewrite H2;rewrite H4;rewrite H13;rewrite H15; simpl; unfold interp_cop; rewrite H3;rewrite H5;simpl.
+      unfold interp_uop; unfold interp_bop; rewrite H10; simpl; rewrite H2;rewrite H4;rewrite H13;rewrite H15; simpl; unfold interp_cop; rewrite H3;rewrite H5;simpl.
       apply bool_impl; intro H28; apply Int63Properties.eqb_spec in H28; subst i4; trivial; apply Bool.eqb_true_iff; trivial.
       
       apply wf_t_atom. apply def_t_atom. 
@@ -296,18 +329,11 @@ Section Checker.
 
     Lemma digit_plus_1_not_0 : (0 == digits+1) = false.
     Proof.
-      apply Int63Properties.eqb_false_complete.
-      apply not_eq_sym.
-      apply Int63Properties.not_0_ltb.
-      apply succ_max_int.
       reflexivity.
     Qed.
 
    Lemma digit_plus_1_not_02 : (digits+1 == 0) = false.
     Proof.
-      apply Int63Properties.eqb_false_complete.
-      apply Int63Properties.not_0_ltb.
-      apply succ_max_int.
       reflexivity.
     Qed.
 
@@ -331,46 +357,12 @@ Section Checker.
 
     Lemma contrap : forall a b, (a = true -> b = true) <-> (b = false -> a = false).
     Proof.
-      intros.
-      split.
-      intros.
-      destruct a.
-      destruct b.
-      trivial.
-      symmetry.
-      apply H.
-      trivial.
-      trivial.
-      intros;destruct a;destruct b.
-      trivial.
-      symmetry.
-      apply H; trivial.
-      trivial.
-      apply H0.
+      intros [ | ] [ | ];split; intros H H0; try (symmetry; apply H);trivial;apply H0.
     Qed.
 
     Lemma bit_eq_false i1 i2: i1 <> i2 -> exists i, bit i1 i <> bit i2 i /\ i < digits = true.
     Proof.
-      intros.
-      rewrite bit_eq in H. 
-      apply not_all_ex_not in H.
-      inversion H.
-      exists x.
-      split.
-      apply H0.
-      assert (digits <= x = true -> (Bool.eqb (bit i1 x) (bit i2 x) = true)).
-      intros.
-      rewrite !bit_M.
-      simpl.
-      trivial.
-      apply H1. apply H1.
-      apply contrap in H1.
-      apply negb_true_iff in H1.
-      rewrite <- H1.
-      rewrite ltb_negb_geb.
-      trivial.
-      rewrite Bool.eqb_false_iff.
-      apply H0.
+      intro H;rewrite bit_eq in H;apply not_all_ex_not in H;inversion H;exists x;split;[apply H0|      assert (digits <= x = true -> (Bool.eqb (bit i1 x) (bit i2 x) = true)) as H1;[intros H2;rewrite !bit_M;simpl;trivial;apply H2|apply contrap in H1;[apply negb_true_iff in H1;rewrite <- H1;rewrite <- ltb_negb_geb;trivial|rewrite Bool.eqb_false_iff;apply H0]]].
     Qed. 
     
     Lemma inf_plus_un : forall a b, (b < max_int) = true -> (a < b) = true -> (a + 1 < b + 1) = true.
@@ -379,38 +371,87 @@ Section Checker.
       rewrite ltb_leb_sub1.
       generalize H2.
       rewrite <- (ltb_leb_add1 (b +1 -1) b a).
-      intro.
+      intro H.
       assert (b = b+1-1).
       rewrite <- to_Z_eq.
       rewrite (to_Z_sub_1 (b+1) 0).
       rewrite (to_Z_add_1 b max_int).
       intuition.
       apply H1.
-      apply succ_max_int.
-      apply H1.
-      rewrite <- H0.
-      apply H.
+      apply succ_max_int;apply H1.
+      rewrite <- H0;apply H.
       apply H2.
-      apply not_0_ltb.
-      apply succ_max_int.
-      apply H1.
+      apply not_0_ltb;apply succ_max_int;apply H1.
     Qed.
 
-    Lemma valid_check_BuildDefInt : forall lits, C.valid rho (check_BuildDefInt lits).
+    Lemma valid_check_BuildDefInt : forall lits i, C.valid rho (check_BuildDefInt lits i).
     Proof.
-      unfold check_BuildDefInt,C.valid; intro lits.
+      unfold check_BuildDefInt,C.valid; intros lits i.
       
-      case_eq (t_form .[ Lit.blit (lits .[ 0])]); intros; auto using C.interp_true.
-      case_eq (t_atom.[i]);intros; auto using C.interp_true.
-      case_eq (b);intros; auto using C.interp_true.
-      case_eq (t_atom.[i0]);intros; auto using C.interp_true.
-      case_eq (c);intros; auto using C.interp_true.
-      case_eq (t_atom .[ i1]);intros; auto using C.interp_true.
-      case_eq (c0);intros; auto using C.interp_true.
-      case_eq ( (length lits == digits + 1) && Lit.is_pos (lits .[ 0]) && Typ.eqb t Typ.Tint &&
-        forallbi
-        (fun i4 l : int =>
-         if i4 == 0
+      case_eq (t_form .[ Lit.blit (lits .[ 0])]); intros i0; auto using C.interp_true; intro H.
+      case_eq (t_atom.[i0]);intros c i1; auto using C.interp_true. intros H0.
+      case_eq c;intro i2;auto using C.interp_true;intro H1.
+      case_eq (t_atom .[ i1]);intros c0 i3; auto using C.interp_true;intros i4 H2.
+      case_eq (c0);intro H3;auto using C.interp_true.
+      case_eq (length lits == 3); intros H9; auto using C.interp_true. 
+      case_eq (t_form .[ Lit.blit (lits .[ 1])]); intros i7; auto using C.interp_true; intro H10.
+      case_eq (t_form .[ Lit.blit (lits .[ 2])]); intros i8; auto using C.interp_true; intro H11.
+      case_eq (t_atom .[ i7]);intros c4 i12; auto using C.interp_true;intro H15.
+      case_eq c4;intro i13;auto using C.interp_true; intro H16.
+      case_eq (t_atom .[ i8]);intros c5 i17; auto using C.interp_true; intro H17.
+      case_eq c5;intro i14;auto using C.interp_true; intro H18.
+      case_eq ((i12 == i3) && (i4 == i17) && (i2 == i13) && (i13 == i14) && (i == i2) &&Lit.is_pos (lits .[ 1]) && Lit.is_pos (lits .[ 2]));intros H23.
+      apply andb_true_iff in H23; destruct H23 as (H23,H31);apply andb_true_iff in H23; destruct H23 as (H23,H26);apply andb_true_iff in H23; destruct H23 as (H23,H27);apply andb_true_iff in H23; destruct H23 as (H23,H28);apply andb_true_iff in H23; destruct H23 as (H23,H29);apply andb_true_iff in H23; destruct H23 as (H23,H30).
+      apply Int63Properties.eqb_spec in H23;apply Int63Properties.eqb_spec in H27;apply Int63Properties.eqb_spec in H28;apply Int63Properties.eqb_spec in H29;apply Int63Properties.eqb_spec in H30;subst i2; subst i13;subst i14;subst i17;subst i12. rewrite <- H1 in H16;rewrite <- H1 in H18; subst c4; subst c5.
+      
+      case_eq (Lit.is_pos (lits.[0]));intro H14.
+      
+      simpl; rewrite orb_false_r; apply orb_true_iff; rewrite orb_true_iff.
+      unfold Lit.interp; rewrite H26; rewrite H14; rewrite Lit.is_pos_neg; rewrite H31; simpl; unfold Var.interp; rewrite !rho_interp; rewrite Lit.blit_neg; rewrite H;rewrite H11;rewrite H10; simpl; unfold Atom.interp_form_hatom; unfold interp_hatom; rewrite !t_interp_wf.
+      rewrite H0;rewrite H17;rewrite H15; simpl; unfold interp_uop; rewrite H1; rewrite !t_interp_wf.
+      rewrite H2; simpl; rewrite !t_interp_wf. 
+      unfold interp_bop; rewrite H3;simpl. unfold apply_binop.
+      Check (interp_atom (t_atom .[ i3])).
+      case_eq (interp_atom (t_atom.[i3])); intros t1' v1 H32.
+      case_eq (interp_atom (t_atom.[i4])); intros t2' v2 H33.
+      case_eq (Typ.cast t1' Typ.Tint); intros k. intro H34.
+      case_eq (Typ.cast t2' Typ.Tint); intros k0. intro H35.
+      simpl;rewrite H34;rewrite H35;simpl.
+
+      unfold bit_rev. rewrite lxor_spec;destruct (bit (k (Typ.interp t_i) v1) i);destruct (bit (k0 (Typ.interp t_i) v2) i);[right;left|left|left|right;right];trivial.
+
+      admit.
+      admit.
+
+      apply wf_t_atom. apply def_t_atom. apply wf_t_atom. apply def_t_atom. apply wf_t_atom. apply def_t_atom. apply wf_t_atom. apply def_t_atom. apply wf_t_atom. apply def_t_atom. apply wf_t_atom. apply def_t_atom. apply wf_t_atom. apply def_t_atom. apply wf_t_atom. apply def_t_atom.
+      
+      simpl; rewrite orb_false_r; apply orb_true_iff; rewrite orb_true_iff.
+      unfold Lit.interp; rewrite H26; rewrite H14; rewrite H31; simpl; unfold Var.interp; rewrite !rho_interp; rewrite H;rewrite H11;rewrite H10; simpl; unfold Atom.interp_form_hatom; unfold interp_hatom; rewrite !t_interp_wf.
+      rewrite H0;rewrite H17;rewrite H15; simpl; unfold interp_uop; rewrite H1; rewrite !t_interp_wf.
+      rewrite H2; simpl; rewrite !t_interp_wf. 
+      unfold interp_bop; rewrite H3;simpl. unfold apply_binop.
+      Check (interp_atom (t_atom .[ i3])).
+      case_eq (interp_atom (t_atom.[i3])); intros t1' v1 H32.
+      case_eq (interp_atom (t_atom.[i4])); intros t2' v2 H33.
+      case_eq (Typ.cast t1' Typ.Tint); intros k. intro H34.
+      case_eq (Typ.cast t2' Typ.Tint); intros k0. intro H35.
+      simpl;rewrite H34;rewrite H35;simpl.
+
+      unfold bit_rev. rewrite lxor_spec;destruct (bit (k (Typ.interp t_i) v1) i);destruct (bit (k0 (Typ.interp t_i) v2) i);[left|right;left|right;right|left];trivial.
+
+      admit.
+      admit.
+
+      apply wf_t_atom. apply def_t_atom. apply wf_t_atom. apply def_t_atom. apply wf_t_atom. apply def_t_atom. apply wf_t_atom. apply def_t_atom. apply wf_t_atom. apply def_t_atom. apply wf_t_atom. apply def_t_atom. apply wf_t_atom. apply def_t_atom. apply wf_t_atom. apply def_t_atom. apply C.interp_true. apply wf_rho.
+
+
+      intros i2 H0.
+      case_eq (c);intros t; auto using C.interp_true;intro H1.
+      case_eq t;intro H00;auto using C.interp_true.
+      case_eq ((length lits == digits + 1) && Lit.is_pos (lits .[ 0]) &&
+      forallbi
+        (fun i6 l : int =>
+         if i6 == 0
          then Lit.is_pos l
          else
           match t_form .[ Lit.blit l] with
@@ -420,21 +461,13 @@ Section Checker.
                   match t_form .[ Lit.blit l2] with
                   | Fatom a2 =>
                       match t_atom .[ a1] with
-                      | Auop (UO_index j) hx1 =>
+                      | Auop (UO_index j) h1' =>
                           match t_atom .[ a2] with
-                          | Auop (UO_index k) hy1 =>
-                              match t_atom .[ hx1] with
-                              | Acop (CO_int x1) =>
-                                  match t_atom .[ hy1] with
-                                  | Acop (CO_int y1) =>
-                                      Lit.is_pos l1 && Lit.is_pos l2 &&
-                                      negb (Lit.is_pos l) && (j == i4 - 1) &&
-                                      (k == j) && (i2 == x1) && (i3 == y1)
-                                  | _ => false
-                                  end 
-                              | _ => false
-                              end
-                          |  _ => false
+                          | Auop (UO_index k) h2' =>
+                              Lit.is_pos l1 && Lit.is_pos l2 &&
+                              negb (Lit.is_pos l) && (j == i6 - 1) &&
+                              (k == j) && (i1 == h1') && (h2' == i2)
+                          | _ => false
                           end
                       | _ => false
                       end
@@ -442,24 +475,30 @@ Section Checker.
                   end
               | _ => false
               end
-          |_ => false
+          | _ => false
           end) lits
-              );intros; auto using C.interp_true.
-      apply andb_true_iff in H6; destruct H6;apply andb_true_iff in H6; destruct H6;apply andb_true_iff in H6; destruct H6; apply Typ.eqb_spec in H8; subst t.
+              );intros H6; auto using C.interp_true.
+      apply andb_true_iff in H6; destruct H6 as (H6,H7);apply andb_true_iff in H6; destruct H6 as (H6,H9); subst t.
 
       rewrite forallbi_spec in H7; unfold C.interp;apply existsb_exists.
  
-      case_eq (i2 == i3);intros.
+      case_eq (i1 == i2);intros H8.
     
-      rewrite Int63Properties.eqb_spec in H6;rewrite Int63Properties.eqb_spec in H8; subst i3.
+      rewrite Int63Properties.eqb_spec in H6;rewrite Int63Properties.eqb_spec in H8; subst i2.
   
       exists (lits.[0]);split.
       apply to_list_In; rewrite H6; reflexivity.
-      unfold Lit.interp; rewrite H9; unfold Var.interp; rewrite rho_interp; rewrite H; simpl;unfold Atom.interp_form_hatom; unfold interp_hatom; rewrite !t_interp_wf. 
+      unfold Lit.interp; rewrite H9; unfold Var.interp; rewrite rho_interp; rewrite H; simpl;unfold Atom.interp_form_hatom; unfold interp_hatom; rewrite !t_interp_wf.   
       rewrite H0; simpl; unfold interp_bop; rewrite H1; simpl; rewrite !t_interp_wf.
-      rewrite H4; rewrite H2; simpl; unfold interp_cop; rewrite H5; rewrite H3; simpl; rewrite Int63Properties.eqb_spec;trivial.
-      
-      apply wf_t_atom. apply def_t_atom. apply wf_t_atom. apply def_t_atom. apply wf_t_atom. apply def_t_atom.
+      case_eq (interp_atom (t_atom.[i1])); intros t' v H32;simpl.
+      case_eq (Typ.cast t' Typ.Tint); intros k. intro H34.
+      simpl. apply Int63Properties.eqb_spec. trivial.
+      admit.
+      apply wf_t_atom. apply def_t_atom. apply wf_t_atom. apply def_t_atom.
+
+      rewrite H4; rewrite H2; simpl; unfold interp_cop;rewrite H5; rewrite H3; simpl; rewrite Int63Properties.eqb_spec;trivial.
+      apply wf_t_atom. apply def_t_atom. apply wf_t_atom. apply def_t_atom. apply wf_t_atom. apply def_t_atom. 
+
 
       apply Int63Properties.eqb_spec in H6. apply Int63Properties.eqb_false_spec in H8; apply bit_eq_false in H8; inversion H8; destruct H10; clear H8.
       exists (lits.[x+1]);split. 
